Protocol/ServiceProvider.fst
@@ -1,29 +1,23 @@
 module Serviceprovider
 
 open Lib
+open SessionManager
 open ContentServer
 open Protocol
 open Saml
 open Crypto
 open Network
 
-val hasValidSession: list (string*string) -> bool
-let hasValidSession cookies = 
-  (* Find AuthenticationKey cookie and validate *)
-  let ak = getStrInTupleList cookies "AuthenticationKey" in
-  if isEmptyStr ak then false 
-  else true (*Should be validated somehow*)
-
 val serviceprovider:  me:prin -> pubkey me -> privkey me ->
                       browser:prin -> idp:prin -> pubkey idp -> unit 
 let serviceprovider me pubk privk browser idp pubkidp = 
-  let reqRes = Recieve browser in (*1*) (*7*)
-  match reqRes with
-  | Get (prin,uri,params,cookies) -> 
+  let req = Recieve browser in (*1*) (*7*)
+  match req with
+  | Get (uri,params,cookies) -> 
 
     (*Check for valid session*)
     if hasValidSession cookies then
-      let resp = Response 200 (getContent uri) [] in
+      let resp = Response (getContent uri) [] in
       Send resp (*8*)
     else (*Create AuthnRequest and send (via client) to idp*)
       (let authnReq = CreateAuthnRequest me idp in 
@@ -32,15 +26,15 @@ let serviceprovider me pubk privk browser idp pubkidp =
       let resp = CreateRedirectResponse idp authnReq sigSP in 
       Send resp (*2*))
 
-  | Post (sp, params, cookies) -> 
-      let msg = getStrInTupleList params "SamlMessage" in
-      let sigIDP = getStrInTupleList params "Signature" in
+  | Post (uri, qparams, fparams, cookies) -> 
+      let msg = getStrInTupleList fparams "SamlMessage" in
+      let sigIDP = getStrInTupleList fparams "Signature" in
       if VerifySignature idp pubkidp msg sigIDP
       then
         (assert(Log idp msg);
-          let ak =  GenerateNonce sp in
-          let resp = Response 200 (getContent "Loggedin") [("AuthenticationKey", ak)] in
+          let ak =  GenerateNonce me in
+          let resp = Response (getContent "Logged-in") [("AuthenticationKey", ak)] in
           Send resp) (*8*)
-      else Send (Response 403 (getErrorPage 403) [])(*8.1*)
+      else Send (ErrorResponse 403 (getErrorPage 403) [])(*8.1*)
   
-  | _ -> Send (Response 400 (getErrorPage 400) [])
+  | _ -> Send (ErrorResponse 400 (getErrorPage 400) [])
