Protocol/SessionManager.fst
@@ -1,0 +1,10 @@
+module SessionManager
+
+open Lib
+
+val hasValidSession: list (string*string) -> bool
+let hasValidSession cookies = 
+  (* Find AuthenticationKey cookie and validate *)
+  let ak = getStrInTupleList cookies "AuthenticationKey" in
+  if isEmptyStr ak then false 
+  else true (*Should be validated somehow*)
