Protocol/identityprovider.fst
@@ -1,26 +1,38 @@
 module Identityprovider
+
+open Lib
+open SessionManager
 open Protocol
+open Saml
+open Crypto
+open Network
 
 val identityprovider: me:prin -> pubkey me -> privkey me 
                       -> browser:prin -> sp:prin -> pubkey sp
                       -> unit
 let identityprovider me pubk privk browser serviceprovider pubksp =
-	
-  let samlreq = Recieve browser in (*3*)
-	match samlreq with
-	| SamlProtocolMessage (idp, msg, sigSP)->  
+	let req = Recieve browser in (*3 & 11*)
+	match req with
+	| Get (prin,uri,params,cookies) ->
+    (*Verify sp signature*)
+    let (msg, sigSP) = GetSamlMessage params in 
+    if VerifySignature serviceprovider pubksp msg sigSP then
+      (assert (Log serviceprovider msg);
+      (*Check for valid session*) 
 
-    if VerifySignature serviceprovider pubksp msg sigSP
-    then
-     (assert (Log serviceprovider msg);
-      let challenge = CreateChallenge browser in
-  
-      let challengeMessage = ChallengeMessage challenge in
-      Send browser challengeMessage (*4*))
-     else Send browser (Failed (400))(*4.1*)
+      if hasValidSession cookies then
+        let token = GetSamlToken cookies in
+        let resp = CreateSamlResponse me privk serviceprovider pubksp token in
+        Send browser resp
+
+      else
+        (let challenge = CreateChallenge browser in
+        let challengeMessage = ChallengeMessage challenge in
+        Send browser challengeMessage (*4*)))
      
-  | Credentials(user, password, challenge') -> 
+     else Send(ErrorResponse 403 (getErrorPage 403) [])(*4.1*) (*TODO*)
 
+  | Post (sp, params, cookies) -> 
     (*Check credentials and challenge*)
     if AuthenticateUser user password challenge'
     then
@@ -32,6 +44,8 @@ let identityprovider me pubk privk browser serviceprovider pubksp =
       let response = SamlProtocolMessage serviceprovider samlresponse sigIDP in
       Send browser response(*6*))
     else Send browser (Failed (400))(*6.3*)
+
+  | _ -> Send (ErrorResponse 400 (getErrorPage 400) [])
 
   | _ -> 
      let samlresponse = CreateSamlResponse me serviceprovider Requester in
